add atoms back in, start getfield, write some examples for stepping

Pyret.v
@@ -3,7 +3,7 @@ Require Import Coq.ZArith.ZArith.
 Require Import Coq.Strings.String.
 
 Module Pyret (Import Atom : ATOM) (Import String : STRING).
-  
+
 Module Atoms := Coq.MSets.MSetList.Make (Atom.Atom).
 Module AtomEnv := Coq.FSets.FMapList.Make (Atom.Atom_as_OT).
 
@@ -21,18 +21,35 @@ Add Relation Atom.atom Atom.eq
   transitivity proved by eq_atom_trans
 as Eq_atom.
 
+
+Ltac destruct_eq_dec a b :=
+  let Eq := fresh "Eq" in
+  destruct (Atom.eq_dec a b) eqn:Eq;
+    try (unfold atom_eq_dec; rewrite Eq); auto;
+    try solve [match goal with
+                 | [ H : ?x <> ?x |- _ ]
+                   => exfalso; apply H; reflexivity end].
+
+
 Definition atom := Atom.t. (* free variables *)
 Definition loc := Atom.atom.
 Definition string := String.string.
 
 Parameter __check__ : atom.
 Parameter __brand__ : atom.
-Axiom distinct_check_brand : ~ Atom.eq __check__ __brand__.
-
 Parameter __has_brand__ : atom.
 Parameter __add_brand__ : atom.
-Axiom distinct_has_add_brand :
-  ~ Atom.eq __has_brand__ __add_brand__.
+
+Axiom check_brand_distinct : __check__ <> __brand__.
+Axiom has_add_distinct : __has_brand__ <> __add_brand__.
+
+(* Tests *)
+Goal (if Atom.eq_dec __check__ __check__ then 5 else 6) = 5.
+destruct_eq_dec __check__ __check__. Defined.
+Goal (if Atom.eq_dec __check__ __brand__ then 5 else 6) = 6.
+destruct_eq_dec __check__ __brand__.
+  exfalso. apply check_brand_distinct; auto. Qed.
+
 
 Inductive brand : Type :=
   | mkbrand : atom -> brand.
@@ -45,7 +62,8 @@ Inductive exp : Type :=
   | eobj : list brand -> list (atom * exp) -> exp
   | ebool : list brand -> bool -> exp
   | ebrand : brand -> exp
-  | edelta : atom -> exp -> exp -> exp.
+  | edelta : atom -> exp -> exp -> exp
+  | egetfield : atom -> exp -> exp.
 Set Elimination Schemes.
 
 Definition exp_rec :=
@@ -67,7 +85,9 @@ Definition exp_rec :=
   (exp_rec_brand :
      forall (b : brand), P (ebrand b))
   (exp_rec_delta :
-     forall (a : atom) (e1 : exp) (e2 : exp), P e1 -> P e2 -> P (edelta a e1 e2)) =>
+     forall (a : atom) (e1 : exp) (e2 : exp), P e1 -> P e2 -> P (edelta a e1 e2))
+  (exp_rec_getfield :
+     forall (a : atom) (e : exp), P e -> P (egetfield a e)) =>
 fix F (e : exp) : P e :=
   match e as e0 return (P e0) with
   | elam bs a e => exp_rec_lam bs a e (F e)
@@ -85,6 +105,7 @@ fix F (e : exp) : P e :=
   | ebool l b => exp_rec_bool l b
   | ebrand b => exp_rec_brand b
   | edelta a e1 e2 => exp_rec_delta a e1 e2 (F e1) (F e2)
+  | egetfield a e => exp_rec_getfield a e (F e)
   end.
 
 Inductive value : exp -> Prop :=
@@ -94,24 +115,27 @@ Inductive value : exp -> Prop :=
   | vbrand : forall b, value (ebrand b).
 
  Hint Constructors value.
-  
+
 SearchAbout sumbool.
 
 SearchAbout pair.
 
+SearchAbout beq_nat.
+
 Fixpoint subst (x:atom) (e:exp) (b:exp) :=
   match b with
     | elam bs arg body =>
-      if Atom.atom_eq_dec x arg
+      if Atom.eq_dec x arg
       then b
       else elam bs arg (subst x e body)
     | eapp fn arg =>
-      eapp (subst x e fn) (subst x e arg) 
+      eapp (subst x e fn) (subst x e arg)
     | eid x' =>
       if Atom.eq_dec x x' then e else b
     | edelta a arg1 arg2 => edelta a (subst x e arg1) (subst x e arg2)
     | eobj bs vs =>
       eobj bs (map (fun v => (fst v, subst x e (snd v))) vs)
+    | egetfield a o => egetfield a (subst x e o)
     | ebool _ _ => b
     | ebrand _ => b
   end.
@@ -123,7 +147,7 @@ Fixpoint subst_many (xs : list atom) (es : list exp) (b : exp) :=
   end.
 
 Inductive eq_brand_i : brand -> brand -> Type :=
-  | eq_brand : forall b1 b2, Atom.eq b1 b2 ->
+  | eq_brand : forall b1 b2, b1 = b2 ->
                              eq_brand_i (mkbrand b1)
                                         (mkbrand b2).
 
@@ -147,7 +171,7 @@ Fixpoint brand_elem (l:list brand) (b:brand) : bool :=
   end.
 
 Fixpoint has_brand (b:brand) (e:exp) : bool :=
-  brand_elem (brand_list e) b.                                      
+  brand_elem (brand_list e) b.
 
 Fixpoint add_brand (b:brand) (e:exp) : exp :=
   if has_brand b e then e else
@@ -166,6 +190,8 @@ Fixpoint snoc {A:Type} (l:list A) (e:A) : list A :=
     | l::ls => l::(snoc ls e)
   end.
 
+SearchAbout nth.
+
 Inductive step : exp -> exp -> Prop :=
   | sapp : forall x e b l,
              value e ->
@@ -176,8 +202,13 @@ Inductive step : exp -> exp -> Prop :=
              Forall (fun x => ~ value x) (map snd es) ->
              ~ value e ->
              step e e' ->
-             step (eobj bs (app vs (cons (a,e) es)))
-                  (eobj bs (app (snoc vs (a,e')) es))
+             step (eobj bs (vs ++ (cons (a,e) es)))
+                  (eobj bs (vs ++ (cons (a,e') es)))
+  | sgetfield : forall bs vs a,
+                  Forall value (map snd vs) ->
+                  In a (map fst vs) ->
+                  step (eobj bs vs)
+                       (GET THE FIELD)
   | sdelta1 : forall a e1 e1' e2,
                step e1 e1' ->
                step (edelta a e1 e2) (edelta a e1' e2)
@@ -193,7 +224,7 @@ Inductive step : exp -> exp -> Prop :=
                   value e ->
                   step (edelta __add_brand__ (ebrand b) e)
                        (add_brand b e).
-                    
+
 
 Parameter __some_brand__ : atom.
 
@@ -214,9 +245,6 @@ Proof.
 Qed.
 
 Definition multistep := multi step.
-  
-Print Atom.Atom_as_OT.
-Hint Rewrite Atom.Atom_as_OT.eq_refl.
 
 Example step_add_has_brand1 :
   multistep
@@ -226,7 +254,9 @@ Example step_add_has_brand1 :
                     (ebool nil true)))
     (ebool nil true).
 Proof.
-  eapply multi_step with (y := (edelta __has_brand__ (ebrand (mkbrand __some_brand__)) (ebool (cons (mkbrand __some_brand__) nil) true))).
+  apply multi_step with
+  (y := (edelta __has_brand__ (ebrand (mkbrand __some_brand__))
+                (ebool (cons (mkbrand __some_brand__) nil) true))).
   apply sdelta2.
   constructor.
   apply sdelta_ab.
@@ -234,7 +264,78 @@ Proof.
   eapply multi_step.
   apply sdelta_hb.
   constructor.
-  simpl. Print Atom.eq_dec. SearchAbout sumbool. rewrite Atom.Atom_as_OT.eq_sym.
+  simpl.
+  destruct_eq_dec __some_brand__ __some_brand__.
   eapply multi_refl.
+Qed.
+
+Parameter f1 : atom.
+Parameter f2 : atom.
+
+SearchAbout fold_right.
+
+Lemma app_split : forall A : Type, forall x y : list A,
+                    x ++ y = fold_right cons y x.
+Proof.
+  intros.
+  induction x.
+  reflexivity.
+  simpl. rewrite IHx. reflexivity.
+Qed.
+
+Lemma fold_cons : forall A : Type, forall x : A, forall y : list A,
+                    x :: y = fold_right cons y [x].
+Proof.
+  intros.
+  reflexivity.
+Qed.
+
+Example step_obj1 :
+  multistep
+    (eobj nil
+          ((f1,ebool nil true)
+             ::(f2, edelta __has_brand__
+                       (ebrand (mkbrand __some_brand__))
+                       (ebool nil true))
+             ::nil))
+    (eobj nil ((f1,ebool nil true)::(f2,ebool nil false)::nil)).
+Proof.
+  rewrite fold_cons.
+  rewrite <- app_split.
+  eapply multi_step with
+  (y := (eobj nil ([(f1, ebool [] true)] ++ [(f2, ebool [] false)] ++ nil))).
+  apply sobj.
+  simpl.
+  constructor.
+  constructor.
+  constructor.
+  constructor.
+  unfold not.
+  intros.
+  inversion H.
+  apply sdelta_hb.
+  constructor.
+  rewrite app_split.
+  simpl.
+  apply multi_refl.
+Qed.
+
+
+Parameter __arg__ : atom.
+
+Example step_app_lam1 :
+  multistep
+    (eapp (elam nil __arg__ (eid __arg__)) (ebool nil true))
+    (ebool nil true).
+Proof.
+  eapply multi_step with (y := (subst __arg__ (ebool nil true) (eid __arg__))).
+  apply sapp.
+  constructor.
+  simpl.
+  destruct_eq_dec __arg__ __arg__.
+  apply multi_refl.
+Qed.
+
+
 
 End Pyret.
